wip, adding ghost effect to reflection typing

ulib/experimental/FStar.Reflection.Typing.fsti
@@ -17,7 +17,9 @@
 module FStar.Reflection.Typing
 
 (** This module defines a typing judgment for (parts of) the total
-    fragment of F*. We are using it in the meta DSL framework as an
+    and ghost fragment of F*.
+    
+    We are using it in the meta DSL framework as an
     official specification for the F* type system.
 
     We expect it to grow to cover more of the F* language.
@@ -150,8 +152,11 @@ let var_as_term (v:var) = pack_ln (Tv_Var (var_as_bv v))
 let binder_of_t_q t q = mk_binder pp_name_default 0 t q
 let mk_abs ty qual t : R.term =  R.pack_ln (R.Tv_Abs (binder_of_t_q ty qual) t)
 let mk_total t = pack_comp (C_Total t)
+let mk_ghost t = pack_comp (C_GTotal t)
 let mk_arrow ty qual t : R.term =
   R.pack_ln (R.Tv_Arrow (binder_of_t_q ty qual) (mk_total t))
+let mk_ghost_arrow ty qual t : R.term =
+  R.pack_ln (R.Tv_Arrow (binder_of_t_q ty qual) (mk_ghost t))
 let bound_var i : R.term = R.pack_ln (R.Tv_BVar (R.pack_bv (make_bv i)))
 
 let open_with_var (x:var) = OpenWith (pack_ln (Tv_Var (var_as_bv x)))
@@ -578,63 +583,73 @@ and freevars_match_returns (m:match_returns_ascription)
     let as_ = freevars_opt as_ freevars in
     b `Set.union` ret `Set.union` as_
 
+//
+// term_ctxt is used to define the equiv relation later,
+//   basically putting two equiv terms in a hole gives equiv terms
+//
+// The abs, arrow, refine, and let cases don't seem right here,
+//   since to prove their equiv, we need to extend gamma for their bodies
+//
+// If this is useful only for app, then may be we should remove it,
+//   and add app rules to the equiv relation itself
+
 [@@ no_auto_projectors]
 noeq
 type term_ctxt =
   | Ctxt_hole            : term_ctxt
   | Ctxt_app_head        : term_ctxt -> argv -> term_ctxt
   | Ctxt_app_arg         : term -> aqualv -> term_ctxt -> term_ctxt
-  | Ctxt_abs_binder      : binder_ctxt -> term -> term_ctxt
-  | Ctxt_abs_body        : binder -> term_ctxt -> term_ctxt
-  | Ctxt_arrow_binder    : binder_ctxt -> comp -> term_ctxt
-  | Ctxt_arrow_comp      : binder -> comp_ctxt -> term_ctxt
-  | Ctxt_refine_sort     : bv -> term_ctxt -> term -> term_ctxt
-  | Ctxt_refine_ref      : bv -> typ -> term_ctxt -> term_ctxt
-  | Ctxt_let_sort        : bool -> list term -> bv -> term_ctxt -> term -> term -> term_ctxt
-  | Ctxt_let_def         : bool -> list term -> bv -> term -> term_ctxt -> term -> term_ctxt
-  | Ctxt_let_body        : bool -> list term -> bv -> term -> term -> term_ctxt -> term_ctxt
-  | Ctxt_match_scrutinee : term_ctxt -> option match_returns_ascription -> list branch -> term_ctxt
+  // | Ctxt_abs_binder      : binder_ctxt -> term -> term_ctxt
+  // | Ctxt_abs_body        : binder -> term_ctxt -> term_ctxt
+  // | Ctxt_arrow_binder    : binder_ctxt -> comp -> term_ctxt
+  // | Ctxt_arrow_comp      : binder -> comp_ctxt -> term_ctxt
+  // | Ctxt_refine_sort     : bv -> term_ctxt -> term -> term_ctxt
+  // | Ctxt_refine_ref      : bv -> typ -> term_ctxt -> term_ctxt
+  // | Ctxt_let_sort        : bool -> list term -> bv -> term_ctxt -> term -> term -> term_ctxt
+  // | Ctxt_let_def         : bool -> list term -> bv -> term -> term_ctxt -> term -> term_ctxt
+  // | Ctxt_let_body        : bool -> list term -> bv -> term -> term -> term_ctxt -> term_ctxt
+  // | Ctxt_match_scrutinee : term_ctxt -> option match_returns_ascription -> list branch -> term_ctxt
 
-and bv_ctxt =
-  | Ctxt_bv : sealed string -> nat -> term_ctxt -> bv_ctxt
+// and bv_ctxt =
+//   | Ctxt_bv : sealed string -> nat -> term_ctxt -> bv_ctxt
 
-and binder_ctxt =
-  | Ctxt_binder : bv -> aqualv -> list term -> term_ctxt -> binder_ctxt
+// and binder_ctxt =
+//   | Ctxt_binder : bv -> aqualv -> list term -> term_ctxt -> binder_ctxt
 
-and comp_ctxt =
-  | Ctxt_total  : term_ctxt -> comp_ctxt
-  | Ctxt_gtotal : term_ctxt -> comp_ctxt
+// and comp_ctxt =
+//   | Ctxt_total  : term_ctxt -> comp_ctxt
+//   | Ctxt_gtotal : term_ctxt -> comp_ctxt
 
 let rec apply_term_ctxt (e:term_ctxt) (t:term) : Tot term (decreases e) =
   match e with
   | Ctxt_hole -> t
   | Ctxt_app_head e arg -> pack_ln (Tv_App (apply_term_ctxt e t) arg)
   | Ctxt_app_arg hd q e -> pack_ln (Tv_App hd (apply_term_ctxt e t, q))
-  | Ctxt_abs_binder b body -> pack_ln (Tv_Abs (apply_binder_ctxt b t) body)
-  | Ctxt_abs_body b e -> pack_ln (Tv_Abs b (apply_term_ctxt e t))
-  | Ctxt_arrow_binder b c -> pack_ln (Tv_Arrow (apply_binder_ctxt b t) c)
-  | Ctxt_arrow_comp b c -> pack_ln (Tv_Arrow b (apply_comp_ctxt c t))
-  | Ctxt_refine_sort b sort phi -> pack_ln (Tv_Refine b (apply_term_ctxt sort t) phi)
-  | Ctxt_refine_ref b sort phi -> pack_ln (Tv_Refine b sort (apply_term_ctxt phi t))
+//   | Ctxt_abs_binder b body -> pack_ln (Tv_Abs (apply_binder_ctxt b t) body)
+//   | Ctxt_abs_body b e -> pack_ln (Tv_Abs b (apply_term_ctxt e t))
+//   | Ctxt_arrow_binder b c -> pack_ln (Tv_Arrow (apply_binder_ctxt b t) c)
+//   | Ctxt_arrow_comp b c -> pack_ln (Tv_Arrow b (apply_comp_ctxt c t))
+//   | Ctxt_refine_sort b sort phi -> pack_ln (Tv_Refine b (apply_term_ctxt sort t) phi)
+//   | Ctxt_refine_ref b sort phi -> pack_ln (Tv_Refine b sort (apply_term_ctxt phi t))
   
-  | Ctxt_let_sort b attrs bv sort def body ->
-    pack_ln (Tv_Let b attrs bv (apply_term_ctxt sort t) def body)
-  | Ctxt_let_def b attrs bv sort def body ->
-    pack_ln (Tv_Let b attrs bv sort (apply_term_ctxt def t) body)
-  | Ctxt_let_body b attrs bv sort def body ->
-    pack_ln (Tv_Let b attrs bv sort def (apply_term_ctxt body t))
+//   | Ctxt_let_sort b attrs bv sort def body ->
+//     pack_ln (Tv_Let b attrs bv (apply_term_ctxt sort t) def body)
+//   | Ctxt_let_def b attrs bv sort def body ->
+//     pack_ln (Tv_Let b attrs bv sort (apply_term_ctxt def t) body)
+//   | Ctxt_let_body b attrs bv sort def body ->
+//     pack_ln (Tv_Let b attrs bv sort def (apply_term_ctxt body t))
     
-  | Ctxt_match_scrutinee sc ret brs ->
-    pack_ln (Tv_Match (apply_term_ctxt sc t) ret brs)
+//   | Ctxt_match_scrutinee sc ret brs ->
+//     pack_ln (Tv_Match (apply_term_ctxt sc t) ret brs)
 
-and apply_binder_ctxt (b:binder_ctxt) (t:term) : Tot binder (decreases b) =
-  let Ctxt_binder binder_bv binder_qual binder_attrs ctxt = b in
-  pack_binder {binder_bv; binder_qual; binder_attrs; binder_sort=apply_term_ctxt ctxt t}
+// and apply_binder_ctxt (b:binder_ctxt) (t:term) : Tot binder (decreases b) =
+//   let Ctxt_binder binder_bv binder_qual binder_attrs ctxt = b in
+//   pack_binder {binder_bv; binder_qual; binder_attrs; binder_sort=apply_term_ctxt ctxt t}
 
-and apply_comp_ctxt (c:comp_ctxt) (t:term) : Tot comp (decreases c) =
-  match c with
-  | Ctxt_total e -> pack_comp (C_Total (apply_term_ctxt e t))
-  | Ctxt_gtotal e -> pack_comp (C_GTotal (apply_term_ctxt e t))
+// and apply_comp_ctxt (c:comp_ctxt) (t:term) : Tot comp (decreases c) =
+//   match c with
+//   | Ctxt_total e -> pack_comp (C_Total (apply_term_ctxt e t))
+//   | Ctxt_gtotal e -> pack_comp (C_GTotal (apply_term_ctxt e t))
 
 noeq
 type constant_typing: vconst -> term -> Type0 = 
@@ -694,53 +709,130 @@ let mk_if (scrutinee then_ else_:R.term) : R.term =
   pack_ln (Tv_Match scrutinee None [(Pat_Constant C_True, then_); 
                                     (Pat_Constant C_False, else_)])
 
+
+// effect and type
+type comp_typ = T.effect_label & typ
+
+let close_comp_typ' (c:comp_typ) (x:var) (i:nat) =
+  fst c, open_or_close_term' (snd c) (CloseVar x) i
+
+let close_comp_typ (c:comp_typ) (x:var) =
+  close_comp_typ' c x 0
+
+let open_comp_typ' (c:comp_typ) (x:var) (i:nat) =
+  fst c, open_or_close_term' (snd c) (open_with_var x) i
+
+let open_comp_typ (c:comp_typ) (x:var) =
+  open_comp_typ' c x 0
+
+let freevars_comp_typ (c:comp_typ) = freevars (snd c)
+
+let mk_comp (c:comp_typ) : R.comp =
+  match fst c with
+  | T.E_Total -> mk_total (snd c)
+  | T.E_Ghost -> mk_ghost (snd c)
+
+let mk_arrow_ct ty qual (c:comp_typ) : R.term =
+  R.pack_ln (R.Tv_Arrow (binder_of_t_q ty qual) (mk_comp c))
+ 
+type relation =
+  | R_Eq
+  | R_Sub
+
+//
+// TODO: support for erasable attribute
+//
+let is_non_informative_name (l:name) : bool =
+  l = R.squash_qn ||
+  l = ["FStar"; "Ghost"; "erased"]
+
+let is_non_informative_fv (f:fv) : bool =
+  is_non_informative_name (inspect_fv f)
+
 [@@ no_auto_projectors]
 noeq
-type typing : env -> term -> term -> Type0 =
+type non_informative : term -> Type0 =
+  | Non_informative_type:
+    u:universe ->
+    non_informative (pack_ln (Tv_Type u))
+  
+  | Non_informative_fv:
+    x:fv{is_non_informative_fv x} ->
+    non_informative (pack_ln (Tv_FVar x))
+  
+  | Non_informative_uinst:
+    x:fv ->
+    us:list universe ->
+    non_informative (pack_ln (Tv_UInst x us))
+
+  | Non_informative_app:
+    t:term ->
+    arg:argv ->
+    non_informative t ->
+    non_informative (pack_ln (Tv_App t arg))
+
+  | Non_informative_total_arrow:
+    t0:term ->
+    q:aqualv ->
+    t1:term ->
+    non_informative t1 ->
+    non_informative (mk_arrow_ct t0 q (T.E_Total, t1))
+  
+  | Non_informative_ghost_arrow:
+    t0:term ->
+    q:aqualv ->
+    t1:term ->
+    non_informative (mk_arrow_ct t0 q (T.E_Ghost, t1))
+    
+
+[@@ no_auto_projectors]
+noeq
+type typing : env -> term -> comp_typ -> Type0 =
   | T_Token :
     g:env ->
     e:term ->
-    t:typ ->
-    squash (FTB.typing_token g e t) ->
-    typing g e t
+    c:comp_typ ->
+    squash (FTB.typing_token g e c) ->
+    typing g e c
 
   | T_Var : 
      g:env ->
      x:bv { Some? (lookup_bvar g (bv_index x)) } ->
-     typing g (pack_ln (Tv_Var x)) (Some?.v (lookup_bvar g (bv_index x)))
+     typing g (pack_ln (Tv_Var x)) (T.E_Total, Some?.v (lookup_bvar g (bv_index x)))
 
   | T_FVar :
      g:env ->
      x:fv { Some? (lookup_fvar g x) } -> 
-     typing g (pack_ln (Tv_FVar x)) (Some?.v (lookup_fvar g x))
+     typing g (pack_ln (Tv_FVar x)) (T.E_Total, Some?.v (lookup_fvar g x))
 
   | T_UInst :
      g:env ->
      x:fv ->
      us:list universe { Some? (lookup_fvar_uinst g x us) } ->
-     typing g (pack_ln (Tv_UInst x us)) (Some?.v (lookup_fvar_uinst g x us))
+     typing g (pack_ln (Tv_UInst x us)) (T.E_Total, Some?.v (lookup_fvar_uinst g x us))
 
   | T_Const:
      g:env ->
      v:vconst ->
      t:term ->
      constant_typing v t ->
-     typing g (constant_as_term v) t
+     typing g (constant_as_term v) (T.E_Total, t)
 
   | T_Abs :
      g:env ->
      x:var { None? (lookup_bvar g x) } ->
      ty:term ->
      body:term { ~(x `Set.mem` freevars body) } ->
-     body_ty:term ->
+     body_c:comp_typ ->
      u:universe ->
      pp_name:pp_name_t ->
      q:aqualv ->
-     typing g ty (tm_type u) ->
-     typing (extend_env g x ty) (open_term body x) body_ty ->
+     typing g ty (T.E_Ghost, tm_type u) ->
+     typing (extend_env g x ty) (open_term body x) body_c ->
      typing g (pack_ln (Tv_Abs (mk_binder pp_name 0 ty q) body))
-              (pack_ln (Tv_Arrow (mk_binder pp_name 0 ty q)
-                                 (mk_total (close_term body_ty x))))
+              (T.E_Total,
+               pack_ln (Tv_Arrow (mk_binder pp_name 0 ty q)
+                                 (mk_comp (close_comp_typ body_c x))))
 
   | T_App :
      g:env ->
@@ -748,10 +840,11 @@ type typing : env -> term -> term -> Type0 =
      e2:term ->
      x:binder ->
      t:term ->
-     typing g e1 (pack_ln (Tv_Arrow x (pack_comp (C_Total t)))) ->
-     typing g e2 (binder_sort x) ->
+     eff:T.effect_label ->
+     typing g e1 (eff, pack_ln (Tv_Arrow x (mk_comp (eff, t)))) ->
+     typing g e2 (eff, binder_sort x) ->
      typing g (pack_ln (Tv_App e1 (e2, binder_qual x)))
-              (open_with t e2)
+              (eff, open_with t e2)
 
   | T_Arrow:
      g:env ->
@@ -762,10 +855,11 @@ type typing : env -> term -> term -> Type0 =
      u2:universe ->
      pp_name:pp_name_t ->
      q:aqualv ->
-     typing g t1 (tm_type u1) ->
-     typing (extend_env g x t1) (open_term t2 x) (tm_type u2) ->
-     typing g (pack_ln (Tv_Arrow (mk_binder pp_name 0 t1 q) (mk_total t2)))
-              (tm_type (u_max u1 u2))
+     eff:T.effect_label ->
+     typing g t1 (T.E_Ghost, tm_type u1) ->
+     typing (extend_env g x t1) (open_term t2 x) (T.E_Ghost, tm_type u2) ->
+     typing g (pack_ln (Tv_Arrow (mk_binder pp_name 0 t1 q) (mk_comp (eff, t2))))
+              (T.E_Total, tm_type (u_max u1 u2))
 
   | T_Refine:
      g:env ->
@@ -774,26 +868,26 @@ type typing : env -> term -> term -> Type0 =
      e:term { ~(x `Set.mem` freevars e) } ->
      u1:universe ->
      u2:universe ->     
-     typing g t (tm_type u1) ->
-     typing (extend_env g x t) (open_term e x) (tm_type u2) ->
-     typing g (pack_ln (Tv_Refine (pack_bv (make_bv 0)) t e)) (tm_type u1)
+     typing g t (T.E_Ghost, tm_type u1) ->
+     typing (extend_env g x t) (open_term e x) (T.E_Ghost, tm_type u2) ->
+     typing g (pack_ln (Tv_Refine (pack_bv (make_bv 0)) t e)) (T.E_Total, tm_type u1)
 
   | T_PropIrrelevance:
      g:env -> 
      e:term -> 
      t:term ->
-     typing g e t ->
-     typing g t tm_prop ->
-     typing g (`()) t
+     typing g e (T.E_Ghost, t) ->
+     typing g t (T.E_Ghost, tm_prop) ->
+     typing g (`()) (T.E_Total, t)
      
   | T_Sub:
      g:env ->
      e:term ->
-     t:term ->
-     t':term ->
-     typing g e t ->
-     sub_typing g t t' ->
-     typing g e t'
+     c:comp_typ ->
+     c':comp_typ ->
+     typing g e c ->
+     sub_comp g c c' ->
+     typing g e c'
 
   | T_If: 
      g:env ->
@@ -803,43 +897,82 @@ type typing : env -> term -> term -> Type0 =
      ty:term ->
      u_ty:universe ->
      hyp:var { None? (lookup_bvar g hyp) /\ ~(hyp `Set.mem` (freevars then_ `Set.union` freevars else_)) } ->
-     typing g scrutinee bool_ty ->
-     typing (extend_env g hyp (eq2 (pack_universe Uv_Zero) bool_ty scrutinee true_bool)) then_ ty ->
-     typing (extend_env g hyp (eq2 (pack_universe Uv_Zero) bool_ty scrutinee false_bool)) else_ ty ->
-     typing g ty (tm_type u_ty) -> //typedness of ty cannot rely on hyp
-     typing g (mk_if scrutinee then_ else_) ty
+     eff:T.effect_label ->
+     typing g scrutinee (eff, bool_ty) ->
+     typing (extend_env g hyp (eq2 (pack_universe Uv_Zero) bool_ty scrutinee true_bool)) then_ (eff, ty) ->
+     typing (extend_env g hyp (eq2 (pack_universe Uv_Zero) bool_ty scrutinee false_bool)) else_ (eff, ty) ->
+     typing g ty (T.E_Ghost, tm_type u_ty) -> //typedness of ty cannot rely on hyp
+     typing g (mk_if scrutinee then_ else_) (eff, ty)
 
-  | T_Match: 
-     g:env ->
-     scrutinee:term ->
-     i_ty:term ->
-     branches:list branch ->
-     ty:term ->
-     typing g scrutinee i_ty ->
-     branches_typing g scrutinee i_ty branches ty ->
-     typing g (pack_ln (Tv_Match scrutinee None branches)) ty
+  // | T_Match: 
+  //    g:env ->
+  //    scrutinee:term ->
+  //    i_ty:term ->
+  //    branches:list branch ->
+  //    ty:term ->
+  //    typing g scrutinee i_ty ->
+  //    branches_typing g scrutinee i_ty branches ty ->
+  //    typing g (pack_ln (Tv_Match scrutinee None branches)) ty
 
-and sub_typing : env -> term -> term -> Type0 =
-  | ST_Equiv:
-      g:env ->
-      t0:term ->
-      t1:term ->
-      equiv g t0 t1 ->
-      sub_typing g t0 t1
+and related : env -> term -> relation -> term -> Type0 =
+  | Rel_equiv:
+    g:env ->
+    t0:term ->
+    t1:term ->
+    rel:relation ->
+    equiv g t0 t1 ->
+    related g t0 rel t1
 
-  | ST_Token: 
-      g:env ->
-      t0:term ->
-      t1:term ->      
-      squash (FTB.subtyping_token g t0 t1) ->
-      sub_typing g t0 t1
+  | Rel_subtyping_token:
+    g:env ->
+    t0:term ->
+    t1:term ->
+    squash (FTB.subtyping_token g t0 t1) ->
+    related g t0 R_Sub t1
 
-  | ST_UnivEq:
-      g:env ->
-      u:universe ->
-      v:universe ->
-      univ_eq u v ->
-      sub_typing g (tm_type u) (tm_type v)
+  | Rel_univ_eq:  // can it be part of the equiv relation?
+    g:env ->
+    u:universe ->
+    v:universe ->
+    rel:relation ->
+    univ_eq u v ->
+    related g (tm_type u) rel (tm_type v)
+
+  | Rel_arrow:
+    g:env ->
+    t1:term ->
+    t2:term ->
+    q:aqualv ->
+    c1:comp_typ ->
+    c2:comp_typ ->
+    rel:relation ->
+    x:var{
+      None? (lookup_bvar g x) /\
+      ~ (x `Set.mem` (freevars_comp_typ c1 `Set.union` freevars_comp_typ c2))
+    } ->
+    related g t2 rel t1 ->
+    related_comp (extend_env g x t2)
+                 (open_comp_typ c1 x)
+                 rel
+                 (open_comp_typ c2 x) ->
+    related g (mk_arrow_ct t1 q c1) rel (mk_arrow_ct t2 q c2)
+
+  | Rel_abs:
+    g:env ->
+    t1:term ->
+    t2:term ->
+    q:aqualv ->
+    e1:term ->
+    e2:term ->
+    x:var{
+      None? (lookup_bvar g x) /\ ~ (x `Set.mem` (freevars e1 `Set.union` freevars e2))
+    } ->
+    related g t1 R_Eq t2 ->
+    related (extend_env g x t1)
+            (open_or_close_term' e1 (open_with_var x) 0)
+            R_Eq
+            (open_or_close_term' e2 (open_with_var x) 0) ->
+    related g (mk_abs t1 q e1) R_Eq (mk_abs t2 q e2)
 
 and equiv : env -> term -> term -> Type0 =
   | EQ_Refl:
@@ -887,7 +1020,32 @@ and equiv : env -> term -> term -> Type0 =
       equiv g t0 t1 ->
       equiv g (apply_term_ctxt ctxt t0) (apply_term_ctxt ctxt t1)
 
-and branches_typing : env -> term -> term -> list branch -> term -> Type0 =
+and related_comp : env -> comp_typ -> relation -> comp_typ -> Type0 =
+  | Relc_typ:
+    g:env ->
+    t0:term ->
+    t1:term ->
+    eff:T.effect_label ->
+    rel:relation ->
+    related g t0 rel t1 ->
+    related_comp g (eff, t0) rel (eff, t1)
+  
+  | Relc_total_ghost:
+    g:env ->
+    t:term ->
+    related_comp g (T.E_Total, t) R_Sub (T.E_Ghost, t)
+
+  | Relc_ghost_total:
+    g:env ->
+    t:term ->
+    non_informative t ->
+    related_comp g (T.E_Ghost, t) R_Sub (T.E_Total, t)
+
+// and branches_typing : env -> term -> term -> list branch -> term -> Type0 =
+
+and sub_typing (g:env) (t1 t2:term) = related g t1 R_Sub t2
+
+and sub_comp (g:env) (c1 c2:comp_typ) = related_comp g c1 R_Sub c2
 
 let bindings = list (var & term)
 let rename_bindings bs x y = FStar.List.Tot.map (fun (v, t) -> (v, rename t x y)) bs
@@ -920,13 +1078,14 @@ val subtyping_token_weakening (g:env)
   : FTB.subtyping_token (extend_env_l g (bs1@(x,t)::bs0)) t0 t1
 
 let simplify_umax (#g:R.env) (#t:R.term) (#u:R.universe)
-                  (d:typing g t (tm_type (u_max u u)))
-   : typing g t (tm_type u)
+                  (d:typing g t (T.E_Total, tm_type (u_max u u)))
+   : typing g t (T.E_Total, tm_type u)
    = let ue
        : univ_eq (u_max u u) u
        = UN_MaxLeq u u (UNLEQ_Refl u)
      in
-     T_Sub _ _ _ _ d (ST_UnivEq _ _ _ ue)
+
+     T_Sub _ _ _ _ d (Relc_typ _ _ _ T.E_Total _ (Rel_univ_eq _ _ _ R_Sub ue))
 
 #push-options "--ifuel 2"
 
@@ -1083,11 +1242,11 @@ and ln'_match_returns (m:match_returns_ascription) (i:int)
 let ln (t:term) = ln' t (-1)
 let ln_comp (c:comp) = ln'_comp c (-1)
 
-val well_typed_terms_are_ln (g:R.env) (e:R.term) (t:R.term) (_:typing g e t)
-  : Lemma (ensures ln e /\ ln t)
+val well_typed_terms_are_ln (g:R.env) (e:R.term) (c:comp_typ) (_:typing g e c)
+  : Lemma (ensures ln e /\ ln (snd c))
 
-val type_correctness (g:R.env) (e:R.term) (t:R.term) (_:typing g e t)
-  : GTot (u:R.universe & typing g t (tm_type u))
+val type_correctness (g:R.env) (e:R.term) (c:comp_typ) (_:typing g e c)
+  : GTot (u:R.universe & typing g (snd c) (T.E_Total, tm_type u))
 
 val binder_offset_pattern_invariant (p:pattern) (s:open_or_close) (i:nat)
   : Lemma (binder_offset_pattern p == binder_offset_pattern (open_or_close_pattern' p s i))
@@ -1336,4 +1495,4 @@ type fstar_top_env = g:fstar_env {
 // g:fstar_top_env -> T.tac ((us, e, t):(univ_names & term & typ){typing (push g us) e t})
 //
 
-type dsl_tac_t = g:fstar_top_env -> T.Tac (r:(R.term & R.typ){typing g (fst r) (snd r)})
+type dsl_tac_t = g:fstar_top_env -> T.Tac (r:(R.term & R.typ){typing g (fst r) (T.E_Total, snd r)})
